38 (#294)

HumanEvalLean/HumanEval38.lean
@@ -1,7 +1,83 @@
 module
+import Std.Tactic.Do
+import Std
+import all Init.Data.Range.Polymorphic.UpwardEnumerable -- UpwardEnumerable.least not exposed
 
-def decode_cyclic : Unit :=
-  ()
+open Std Std.Do
+
+def encodeVector {n : Nat} (arr : Vector α n) : Vector α n := Id.run do
+  let mut vec : Vector α n := arr
+
+  for h : i in (*...n / 3) do
+    let tmp := vec[3 * i]
+    vec := vec.set (3 * i) vec[3 * i + 1]
+    vec := vec.set (3 * i + 1) vec[3 * i + 2]
+    vec := vec.set (3 * i + 2) tmp
+
+  return vec
+
+def encodeArray (arr : Array α) : Array α :=
+  (encodeVector arr.toVector).toArray
+
+def encodeCyclic (s : String) : String :=
+  String.ofList (encodeArray s.toList.toArray).toList
+
+def decodeCyclic (s : String) : String :=
+  String.ofList (encodeArray (encodeArray s.toList.toArray)).toList
+
+theorem List.Cursor.length_prefix_le {l : List α} (c : l.Cursor) : c.prefix.length ≤ l.length := by
+  have := congrArg List.length c.property
+  simp at this
+  omega
+
+theorem Nat.eq_add_of_toList_rio_eq_append_cons {a : Nat} {pref cur suff}
+    (h : (*...a).toList = pref ++ cur :: suff) :
+    cur = pref.length := by
+  have := Rio.eq_succMany?_of_toList_eq_append_cons h
+  simpa [PRange.UpwardEnumerable.least, PRange.least?] using this
+
+set_option mvcgen.warning false in
+theorem getElem_encodeVector {arr : Vector α n} {i : Nat} {hi} :
+    (encodeVector arr)[i]'hi =
+      if h : i < 3 * (arr.size / 3) then
+        if hmod : i % 3 = 2 then
+          arr[i - 2]
+        else
+          arr[i + 1]
+      else
+        arr[i]'(by simp_all) := by
+  generalize hwp : encodeVector arr = wp
+  apply Id.of_wp_run_eq hwp
+  mvcgen invariants
+  · ⇓⟨xs, vec⟩ =>
+    ⌜∀ (i : Nat) (hi : i < n), vec[i] =
+      have : xs.prefix.length ≤ n / 3 := by simpa using xs.length_prefix_le
+      if h : i < 3 * xs.prefix.length then
+        if hmod : i % 3 = 2 then
+          arr[i - 2]
+        else
+          arr[i + 1]
+      else
+        arr[i]'(by simp_all)⌝
+  with
+    grind [Nat.eq_add_of_toList_rio_eq_append_cons, Rio.length_toList, Nat.size_rio]
+
+@[simp]
+theorem encodeVector_encodeVector_encodeVector {arr : Vector α n} :
+    encodeVector (encodeVector (encodeVector arr)) = arr := by
+  grind [getElem_encodeVector]
+
+@[simp]
+theorem encodeArray_encodeArray_encodeArray {arr : Array α} :
+    encodeArray (encodeArray (encodeArray arr)) = arr := by
+  ext
+  · simp [encodeArray]
+  · simp only [encodeArray, Vector.getElem_toArray, getElem_encodeVector, Vector.size_toArray,
+      Vector.getElem_mk, Nat.reduceSubDiff]
+    grind
+
+theorem decodeCyclic_encodeCyclic {s : String} : decodeCyclic (encodeCyclic s) = s := by
+  simp [decodeCyclic, encodeCyclic]
 
 /-!
 ## Prompt
